Some progress in commute.v (#17)
* (Re)defined consistency

* Redefined decision as function (instead of relation).

* Cleaned up some stuff.

* Completed merge.

* Final clean-up

commute.v
@@ -3,17 +3,16 @@ Import List Notations.
 From Casper 
 Require Import preamble ListExtras ListSetExtras RealsExtras protocol common definitions vlsm indexed_vlsm.
 
-(* All this should change with Mihai's PR
-
 (* 3.1 Decisions on consensus values *) 
 
 (* Need to add consensus values (and decision functions) to VLSM definitions? *) 
-Class VLSM_plus `{VLSM} :=
+Class consensus_values :=
   { C : Type;
     about_C : exists (c1 c2 : C), c1 <> c2;
   }.
 
-Definition decision `{VLSM_plus} : Type := state -> option C -> Prop. 
+Definition decision {message} (S : LSM_sig message) {CV : consensus_values} : Type
+  := @state _ S -> option C.
 
 (* 3.2.1 Decision finality *)
 (* Program Definition prot_state0 `{VLSM} : protocol_state := 
@@ -24,75 +23,147 @@ Next Obligation.
   constructor.
 Defined. *)
 
-Definition final `{VLSM_plus} : decision -> Prop :=
-  fun (D : decision) => forall (tr : protocol_trace), 
+Definition final {message} {S : LSM_sig message} (V : @VLSM message S) {CV : consensus_values}
+  : decision S -> Prop :=
+  fun (D : decision S) => forall (tr : protocol_trace V), 
       forall (n1 n2 : nat) (s1 s2 : state) (c1 c2 : C),
         (trace_nth (proj1_sig tr) n1 = Some s1) ->
         (trace_nth (proj1_sig tr) n2 = Some s2) ->
-        (D s1 (Some c1)) ->
-        (D s2 (Some c2)) ->
+        (D s1 = (Some c1)) ->
+        (D s2 = (Some c2)) ->
         c1 = c2.
 
 (* 3.2.2 Decision consistency *)
-Definition in_trace `{VLSM} : state -> Trace -> Prop :=
-  fun (s : state) (tr : Trace) => exists (n : nat), trace_nth tr n = Some s.
 
 Definition consistent
-  {index : Set}
-  {message : Type}
-  `{VLSM_plus}
-  (IS : index -> LSM_sig message)
+  {CV : consensus_values}
+  {index : Set} `{Heqd : EqDec index}
+  {message : Type} 
+  {IS : index -> LSM_sig message}
   (IM : forall i : index, @VLSM message (IS i))
-  (ID : index -> decision)
-  : Prop
+  (Hi : index)
+  (constraint : indexed_label IS -> indexed_state IS * option (indexed_proto_message IS) -> Prop)
+  (X := indexed_vlsm_constrained Hi IS IM constraint)
+  (ID : forall i : index, decision (IS i)) : Prop
   :=
-    (* Assuming we want traces of the overall protocol *)
-    forall (tr : protocol_trace) (s : state),
-      in_trace s (proj1_sig tr) ->
-      forall (n1 n2 j k : index),
-      exists (c1 c2 : C),
-        (ID n1) s (Some c1) -> (ID n2) s (Some c2) ->
-        forall (c : C),
-          (ID n1) s (Some c) <-> (ID n2) s (Some c).       
-  
+    forall (tr : @protocol_trace _ _ X), 
+    forall (n1 n2 : nat),
+    forall (j k : index),
+    forall (s1 s2 : @state _ (sign X)),
+    forall (c1 c2 : C),
+    j <> k ->
+    trace_nth (proj1_sig tr) n1 = (Some s1) ->
+    trace_nth (proj1_sig tr) n2 = (Some s2) ->
+    (ID j) (@s1 j) = (Some c1) -> 
+    (ID k) (@s2 k) = (Some c2) -> 
+    c1 = c2.
+
+(** The following is an attempt to include finality in the definition of consistency by dropping the requirement 
+    that (j <> k). **)
+
+Definition final_and_consistent
+  {CV : consensus_values}
+  {index : Set} `{Heqd : EqDec index}
+  {message : Type} 
+  {IS : index -> LSM_sig message}
+  (IM : forall i : index, @VLSM message (IS i))
+  (Hi : index)
+  (constraint : indexed_label IS -> indexed_state IS * option (indexed_proto_message IS) -> Prop)
+  (X := indexed_vlsm_constrained Hi IS IM constraint)
+  (ID : forall i : index, decision (IS i)) : Prop
+  :=
+    forall (tr : @protocol_trace _ _ X), 
+    forall (n1 n2 : nat),
+    forall (j k : index),
+    forall (s1 s2 : @state _ (sign X)),
+    forall (c1 c2 : C),
+    trace_nth (proj1_sig tr) n1 = (Some s1) ->
+    trace_nth (proj1_sig tr) n2 = (Some s2) ->
+    (ID j) (@s1 j) = (Some c1) -> 
+    (ID k) (@s2 k) = (Some c2) -> 
+    c1 = c2.
+
+Lemma final_and_consistent_implies_final
+  {CV : consensus_values}
+  {index : Set} `{Heqd : EqDec index}
+  {message : Type} 
+  {IS : index -> LSM_sig message}
+  (IM : forall i : index, @VLSM message (IS i))
+  (Hi : index)
+  (constraint : indexed_label IS -> indexed_state IS * option (indexed_proto_message IS) -> Prop)
+  (X := indexed_vlsm_constrained Hi IS IM constraint)
+  (ID : forall i : index, decision (IS i))
+  : 
+    final_and_consistent IM Hi constraint ID ->
+    forall i : index, final (indexed_vlsm_constrained_projection Hi IS IM constraint i) (ID i).
+
+Proof.
+  unfold final_and_consistent.
+  intros.
+  unfold final.
+  intros.
+  Admitted.
+
 (* 3.3.1 Initial protocol state bivalence *)
-Definition bivalent `{VLSM_plus} : decision -> Prop :=
-  fun (D : decision) =>
+Definition bivalent {message} {S : LSM_sig message} (V : @VLSM message S) {CV : consensus_values} : decision S -> Prop :=
+  fun (D : decision S) =>
     (* All initial states decide on None *) 
     (forall (s0 : state),
       initial_state_prop s0 ->
-      D s0 None) /\
+      D s0 = None) /\
     (* Every protocol trace (already beginning from an initial state) contains a state deciding on each consensus value *) 
-    (forall (c : C) (tr : protocol_trace),
-        exists (s : state) (n : nat), 
-          (trace_nth (proj1_sig tr) n) = Some s /\ D s (Some c)).
+    (forall (c : C) ,
+        exists (tr : protocol_trace V) (s : state) (n : nat), 
+          (trace_nth (proj1_sig tr) n) = Some s /\ D s = (Some c)).
 
 (* 3.3.2 No stuck states *) 
-(* Definition stuck_free `{VLSM_plus} : decision -> Prop :=
-  fun (D : decision) =>
-    (exists (s : state),
-        forall (tr : trace) (n : nat),
-            D (Trace_nth tr n) None) -> False. 
- *)
+
+Definition stuck_free {message} {S : LSM_sig message} (V : @VLSM message S) {CV : consensus_values} : decision S -> Prop :=
+  fun (D : decision S) =>
+    (forall (s : state),
+        exists (tr : protocol_trace V) 
+               (decided_state : state)
+               (n_s n_decided : nat)
+               (c : C),
+       trace_nth (proj1_sig tr) n_s = Some s /\
+       trace_nth (proj1_sig tr) n_decided = Some decided_state /\
+       n_decided >= n_s /\
+       D decided_state = Some c).
+ 
 (* 3.3.3 Protocol definition symmetry *) 
 (* How do we formalize this property set-theoretically? *)
-Definition behavior `{VLSM_plus} : decision -> Prop := fun _ => True. 
-Definition symmetric `{VLSM_plus} :=
-  forall (D : decision),
-  exists (f : decision -> decision),
+
+Definition behavior 
+  {message} 
+  {S : LSM_sig message} 
+  {V : @VLSM message S} 
+  {CV : consensus_values} : decision S -> Prop := 
+  fun _ => True.
+
+Definition symmetric 
+  {message}
+  {S : LSM_sig message}
+  (V : @VLSM message S)
+  {CV : consensus_values} : decision S -> Prop :=
+  fun (D : decision S) =>
+  exists (f : decision S -> decision S),
     behavior D = behavior (f D).
 
-(* 3.4 Liveness *) 
-Definition live `{VLSM_plus} : (nat -> VLSM_plus) -> (nat -> decision) -> Prop :=
-  fun (IS : nat -> VLSM_plus) (ID : nat -> decision) =>
-    (* Here we want traces starting at the initial states *)
-    forall (tr : protocol_trace) (s : state) (n : nat),
-      trace_nth (proj1_sig tr) n = Some s ->
-      exists (i n : nat) (c : C),
-        (ID i) s (Some c). 
+Definition live 
+  {CV : consensus_values}
+  {index : Set} `{Heqd : EqDec index}
+  {message : Type} 
+  {IS : index -> LSM_sig message}
+  (IM : forall i : index, @VLSM message (IS i))
+  (Hi : index)
+  (constraint : indexed_label IS -> indexed_state IS * option (indexed_proto_message IS) -> Prop)
+  (X := indexed_vlsm_constrained Hi IS IM constraint)
+  (ID : forall i : index, decision (IS i)) : Prop
+  :=
+  forall (tr : @protocol_trace _ _ X),
+    @complete_trace_prop _ _ _ _ _ X tr -> 
+    exists (s : @state _ (sign X)) (n : nat) (i : index) (c : C), 
+      trace_nth (proj1_sig tr) n = Some s /\
+      (ID i) (@s i) = Some c.
 
-(* Section 4 *) 
-
-
-*)
-  
+(* Section 4 *)
